theories/Theorems/NormalForm.v
@@ -1,0 +1,122 @@
+Require Import Nat.
+Require Import PeanoNat.
+Require Import Logic.Decidable.
+Require Import Coq.Arith.Compare_dec.
+Require Import Definitions.Ident.
+Require Import Definitions.Term.
+Require Import Definitions.Type.
+Require Import Definitions.Typing.
+Require Import Definitions.Reduction.
+Require Import Theorems.Reduction.
+Require Import Theorems.ChurchRosser.
+
+Require Import ssreflect ssrfun ssrbool.
+
+Open Scope system_t_term_scope.
+Open Scope system_t_type_scope.
+
+Lemma normal_form_reduction_star {e f : termT} :
+    normal_form e -> (e ->* f) -> e = f.
+Proof.
+  intros Hnf Hred.
+  destruct Hred as [n Hn].
+  inversion Hn.
+  - reflexivity.
+  - destruct Hnf.
+    exists f0.
+    assumption.
+Qed.
+
+Lemma normal_form_equivalence {e f : termT} :
+    normal_form e -> normal_form f ->
+    e === f -> e = f.
+Proof.
+  intros Hnfe Hnff Hequiv.
+  rewrite equivalence_reduction_star in Hequiv.
+  destruct Hequiv as [g [Hredeg Hredfg]].
+  apply (normal_form_reduction_star Hnfe) in Hredeg.
+  apply (normal_form_reduction_star Hnff) in Hredfg.
+  rewrite Hredeg.
+  rewrite Hredfg.
+  reflexivity.
+Qed.
+
+Lemma normal_form_fvarT {f : fident} :
+    normal_form (fvarT f).
+Proof.
+  intro Hred.
+  destruct Hred as [g Hred].
+  inversion Hred.
+Qed.
+
+Lemma normal_form_bvarT {n : nat} :
+    normal_form (bvarT n).
+Proof.
+  intro Hred.
+  destruct Hred as [g Hred].
+  inversion Hred.
+Qed.
+
+Lemma normal_form_absT {e : termT} :
+    normal_form e ->
+    normal_form (absT e).
+Proof.
+  intros Hnf Hred.
+  destruct Hred as [g Hred].
+  inversion Hred.
+  apply Hnf.
+  eexists.
+  eauto.
+Qed.
+
+Lemma normal_form_trueT :
+    normal_form trueT.
+Proof.
+  intro Hred.
+  destruct Hred as [g Hred].
+  inversion Hred.
+Qed.
+
+Lemma normal_form_falseT :
+    normal_form falseT.
+Proof.
+  intro Hred.
+  destruct Hred as [g Hred].
+  inversion Hred.
+Qed.
+
+Lemma normal_form_oT :
+    normal_form oT.
+Proof.
+  intro Hred.
+  destruct Hred as [g Hred].
+  inversion Hred.
+Qed.
+
+Lemma normal_form_sT {e : termT} :
+    normal_form e ->
+    normal_form (sT e).
+Proof.
+  intros Hnf Hred.
+  destruct Hred as [g Hred].
+  inversion Hred.
+  apply Hnf.
+  eexists.
+  eauto.
+Qed.
+
+Lemma normal_form_bool_as_boolT {b : bool} :
+    normal_form (bool_as_boolT b).
+Proof.
+  destruct b.
+  - exact normal_form_trueT.
+  - exact normal_form_falseT.
+Qed.
+
+Lemma normal_form_nat_as_natT {n : nat} :
+    normal_form (nat_as_natT n).
+Proof.
+  induction n.
+  - exact normal_form_oT.
+  - eauto using normal_form_sT.
+Qed.
