theories/Theorems/StrongNormalization.v
@@ -1,0 +1,102 @@
+Require Import Nat.
+Require Import PeanoNat.
+Require Import Logic.Decidable.
+Require Import Coq.Arith.Compare_dec.
+Require Import Definitions.Ident.
+Require Import Definitions.Term.
+Require Import Definitions.Type.
+Require Import Definitions.Typing.
+Require Import Definitions.Reduction.
+Require Import Theorems.Reduction.
+
+Require Import ssreflect ssrfun ssrbool.
+
+Open Scope system_t_term_scope.
+Open Scope system_t_type_scope.
+
+Lemma normal_form_strongly_normalizing {e : termT} :
+    normal_form e -> strongly_normalizing e.
+Proof.
+  intro Hnf.
+  constructor.
+  intros f Hred.
+  destruct Hnf.
+  exists f.
+  assumption.
+Qed.
+
+Lemma strongly_normalizing_appT_inv_l {e f : termT} :
+    strongly_normalizing (appT e f) ->
+    strongly_normalizing e.
+Proof.
+  generalize (eq_refl (appT e f)).
+  pattern (appT e f) at -1.
+  generalize (appT e f) at -2.
+  simpl.
+  move=> g Heq Hsn.
+  rewrite <- Heq in Hsn.
+  move: Heq.
+  move: e f.
+  induction Hsn;
+  move=> e f Heq.
+  constructor.
+  move=> h Hred.
+  eapply (H0 (appT h f)).
+  - rewrite Heq.
+    unfold "1<-" in Hred.
+    unfold "1<-".
+    eauto using one_reduction.
+  - reflexivity.
+Qed.
+
+Lemma strongly_normalizing_appT_inv_r {e f : termT} :
+    strongly_normalizing (appT e f) ->
+    strongly_normalizing f.
+Proof.
+  generalize (eq_refl (appT e f)).
+  pattern (appT e f) at -1.
+  generalize (appT e f) at -2.
+  simpl.
+  move=> g Heq Hsn.
+  rewrite <- Heq in Hsn.
+  move: Heq.
+  move: e f.
+  induction Hsn;
+  move=> e f Heq.
+  constructor.
+  move=> h Hred.
+  eapply (H0 (appT e h)).
+  - rewrite Heq.
+    unfold "1<-" in Hred.
+    unfold "1<-".
+    eauto using one_reduction.
+  - reflexivity.
+Qed.
+
+Fixpoint reducibility_candidate (t : typeT) : termT -> Prop :=
+  match t with
+  | boolT =>
+    fun e =>
+      strongly_normalizing e /\ (exists b : bool, e ->* bool_as_boolT b)
+  | natT =>
+    fun e =>
+      strongly_normalizing e /\ (exists n : nat, e ->* nat_as_natT n)
+  | tvarT t =>
+    strongly_normalizing
+  | funT t u =>
+    fun e =>
+      forall f : termT,
+      reducibility_candidate t f ->
+      reducibility_candidate u (appT e f)
+  end.
+
+Lemma reducibility_candidate_sat1 {t :  typeT} {e f : termT} :
+    reducibility_candidate t (e[O <- f]) ->
+    strongly_normalizing f ->
+    reducibility_candidate t (appT (absT e) f).
+Proof.
+  move: e f.
+  induction t;
+  simpl;
+  move=> e f Hred Hsn.
+Admitted.
