theories/Theorems/TermExample.v
@@ -1,0 +1,139 @@
+Require Import Nat.
+Require Import PeanoNat.
+Require Import Logic.Decidable.
+Require Import Coq.Arith.Compare_dec.
+Require Import Definitions.Ident.
+Require Import Definitions.Term.
+Require Import Definitions.Type.
+Require Import Definitions.Typing.
+Require Import Definitions.Reduction.
+Require Import Theorems.Reduction.
+
+Require Import ssreflect ssrfun ssrbool.
+
+Open Scope system_t_term_scope.
+Open Scope system_t_type_scope.
+
+Definition type_bool_as_boolT (b : bool) :
+    |- bool_as_boolT b :T boolT :=
+  match b with
+  | true => trueT_ax Context.empty
+  | _ => falseT_ax Context.empty
+  end.
+
+Fixpoint type_nat_as_natT (n : nat) :
+    |- (nat_as_natT n) :T natT :=
+  match n with
+  | O => oT_ax Context.empty
+  | S n =>
+    sT_el Context.empty (nat_as_natT n) (type_nat_as_natT n)
+  end.
+
+Definition idT : termT := absT (bvarT O).
+
+Definition notT : termT :=
+  absT (iteT (bvarT O) falseT trueT).
+
+Definition andT : termT :=
+  absT (absT (iteT (bvarT O) (bvarT 1) falseT)).
+
+Definition orT : termT :=
+  absT (absT (iteT (bvarT O) trueT (bvarT 1))).
+
+Lemma type_idT {t : typeT} :
+    |- idT :T t ->T t.
+Proof.
+  unfold idT.
+  apply absT_in.
+  unfold Context.bpush.
+  simpl.
+  apply bvarT_ax.
+  unfold Context.bMapsTo.
+  simpl.
+  reflexivity.
+Qed.
+
+Lemma type_notT :
+    |- notT :T boolT ->T boolT.
+Proof.
+  apply absT_in.
+  unfold Context.bpush;
+  unfold Context.empty;
+  simpl.
+  apply iteT_el;
+  eauto using derivation.
+  apply bvarT_ax.
+  unfold Context.bMapsTo.
+  simpl.
+  reflexivity.
+Qed.
+
+Lemma type_andT :
+    |- andT :T boolT ->T boolT ->T boolT.
+Proof.
+  apply absT_in.
+  apply absT_in.
+  unfold Context.empty;
+  unfold Context.bpush;
+  simpl.
+  apply iteT_el;
+  eauto using derivation;
+  apply bvarT_ax;
+  unfold Context.bMapsTo;
+  simpl;
+  reflexivity.
+Qed.
+
+Lemma type_orT :
+    |- orT :T boolT ->T boolT ->T boolT.
+Proof.
+  apply absT_in.
+  apply absT_in.
+  unfold Context.empty;
+  unfold Context.bpush;
+  simpl.
+  apply iteT_el;
+  eauto using derivation;
+  apply bvarT_ax;
+  unfold Context.bMapsTo;
+  simpl;
+  reflexivity.
+Qed.
+
+Lemma idT_one_reduction {e : termT} : appT idT e ->1 e.
+Proof.
+  eauto using one_reduction.
+Qed.
+
+Lemma idT_spec {e : termT} : appT idT e ->* e.
+Proof.
+  exact (one_reduction_reduction_star idT_one_reduction).
+Qed.
+
+Lemma noT_spec {b : bool} :
+    appT notT (bool_as_boolT b) ->* bool_as_boolT (~~ b).
+Proof.
+  exists 2.
+  destruct b;
+  eauto using one_reduction, reduction.
+Qed.
+
+Lemma andT_spec {b c : bool} :
+    appT (appT andT (bool_as_boolT b)) (bool_as_boolT c) ->*
+    bool_as_boolT (b && c).
+Proof.
+  exists 3.
+  destruct b;
+  destruct c;
+  eauto using one_reduction, reduction.
+Qed.
+
+Lemma orT_spec {b c : bool} :
+    appT (appT orT (bool_as_boolT b)) (bool_as_boolT c) ->*
+    bool_as_boolT (b || c).
+Proof.
+  exists 3.
+  destruct b;
+  destruct c;
+  eauto using one_reduction, reduction.
+Qed.
